Morph/Tests/Typing.lean
@@ -11,16 +11,16 @@ section TypeSystemTests
   open Morph.Core
   open Morph.Syntax
 
-  example : inferType [] (.lit (.int 42)) = some .intType := by
+  example : inferType [] [] (.lit (.int 42)) = some .intType := by
     simp [inferType]
 
-  example : inferType [] (.lit (.bool true)) = some .boolType := by
+  example : inferType [] [] (.lit (.bool true)) = some .boolType := by
     simp [inferType]
 
-  example : inferType [] (.lit .unit) = some .unitType := by
+  example : inferType [] [] (.lit .unit) = some .unitType := by
     simp [inferType]
 
-  example : inferType [("x", .intType)] (.var { name := "x" }) = some .intType := by
+  example : inferType [] [("x", .intType)] (.fvar "x") = some .intType := by
     unfold inferType lookupTyp
     simp [Option.map]
 
